Move old files in separate folder

io/IIO.fst
@@ -2,7 +2,7 @@ module IIO
 
 open FStar.Tactics
 open ExtraTactics
-open FStar.Calc
+open FStar.Ghost
 
 open IO.Sig
 open IO.Sig.Call
@@ -43,50 +43,213 @@ val dm_iio_subcomp :
   Pure (dm_iio a wp2) (hist_ord wp2 wp1) (fun _ -> True)
 let dm_iio_subcomp a wp1 wp2 f = dm_subcomp iio_cmds iio_sig event iio_wps a wp1 wp2 f
 
-let dm_iio_if_then_else a wp1 wp2 f g b = dm_if_then_else iio_cmds iio_sig event iio_wps a wp1 wp2 f g b
+(** * The IIO effect indexed by actions **)
 
-val lift_pure_dm_iio :
+(** ** Types **)
+
+(** **** Tree **)
+type tree (a: Type) =
+  | Leaf : tree a
+  | EmptyNode: left: tree a -> right: tree a -> tree a
+  | Node: data: a -> left: tree a -> right: tree a -> tree a
+
+let root (t:(tree 'a){Node? t}) = Node?.data t
+let eleft (t:(tree 'a){EmptyNode? t}) = EmptyNode?.left t
+let eright (t:(tree 'a){EmptyNode? t}) = EmptyNode?.right t
+let left (t:(tree 'a){Node? t}) = Node?.left t
+let right (t:(tree 'a){Node? t}) = Node?.right t
+
+let rec equal_trees (t1:tree 'a) (t2:tree 'a) =
+  match t1, t2 with
+  | Leaf, Leaf -> True
+  | EmptyNode lhs1 rhs1, EmptyNode lhs2 rhs2 -> equal_trees lhs1 lhs2 /\ equal_trees rhs1 rhs2
+  | Node x lhs1 rhs1, Node y lhs2 rhs2 -> x == y /\ equal_trees lhs1 lhs2 /\ equal_trees rhs1 rhs2
+  | _, _ -> False
+
+let rec map_tree (t:tree 'a) (f:'a -> 'b) : tree 'b =
+  match t with
+  | Leaf -> Leaf 
+  | EmptyNode lhs rhs -> EmptyNode (map_tree lhs f) (map_tree rhs f)
+  | Node x lhs rhs -> Node (f x) (map_tree lhs f) (map_tree rhs f)
+
+(** **** Flag **)
+noeq
+type tflag = | NoActions | GetTraceActions | IOActions | AllActions
+
+let rec satisfies (m:iio 'a) (flag:tflag) =
+match flag, m with
+| AllActions,   _                     -> True
+| _,            Return x              -> True
+| _,            PartialCall pre k     -> forall r. satisfies (k r) flag
+| NoActions,    _                     -> False
+| GetTraceActions, Call GetTrace arg k   -> forall r. satisfies (k r) flag
+| GetTraceActions, Call cmd arg k        -> False
+| IOActions,    Call GetTrace arg k   -> False
+| IOActions,    Call cmd arg k        -> forall r. satisfies (k r) flag
+
+let (+) (flag1:tflag) (flag2:tflag) = 
+  match flag1, flag2 with
+  | NoActions, NoActions -> NoActions
+  | NoActions, fl -> fl
+  | fl, NoActions -> fl
+  | GetTraceActions, GetTraceActions -> GetTraceActions
+  | IOActions, IOActions -> IOActions
+  | _, _ -> AllActions
+
+let (<=) (flag1:tflag) (flag2:tflag) =
+  match flag1, flag2 with
+  | NoActions, _ -> True
+  | GetTraceActions, NoActions -> False
+  | GetTraceActions, _ -> True
+  | IOActions, NoActions -> False
+  | IOActions, GetTraceActions -> False
+  | IOActions, _ -> True
+  | AllActions, AllActions -> True
+  | AllActions, _ -> False
+
+(** ** Defining F* Effect **)
+
+type dm_giio (a:Type) (flag:erased tflag) (wp:hist a) = t:(dm_iio a wp){t `satisfies` flag} 
+
+let dm_giio_theta #a = theta #a #iio_cmds #iio_sig #event iio_wps
+
+let dm_giio_return (a:Type) (x:a) : dm_giio a NoActions (hist_return x) by (compute ()) =
+  dm_iio_return a x
+
+val dm_giio_bind  : 
   a: Type ->
-  w: pure_wp a ->
-  f: (eqtype_as_type unit -> PURE a w) ->
-  Tot (dm_iio a (wp_lift_pure_hist w))
-let lift_pure_dm_iio = lift_pure_dm iio_cmds iio_sig event iio_wps
+  b: Type ->
+  flag_v : tflag ->
+  flag_f : tflag ->
+  wp_v: Hist.hist a ->
+  wp_f: (_: a -> Hist.hist b) ->
+  v: dm_giio a flag_v wp_v ->
+  f: (x: a -> dm_giio b flag_f (wp_f x)) ->
+  Tot (dm_giio b (flag_v + flag_f) (hist_bind wp_v wp_f))
+let dm_giio_bind a b flag_v flag_f wp_v wp_f v f : (dm_giio b (flag_v + flag_f) (hist_bind wp_v wp_f)) = 
+  let r = dm_iio_bind a b wp_v wp_f v f in
+  assume (v `satisfies` flag_v /\ (forall x. f x `satisfies` flag_f) ==> r `satisfies` (flag_v + flag_f));
+  r
 
-(*
-[@@allow_informative_binders]
+val dm_giio_subcomp : 
+  a: Type ->
+  flag1 : tflag ->
+  flag2 : tflag ->
+  wp1: hist a ->
+  wp2: hist a ->
+  f: dm_giio a flag1 wp1 ->
+  Pure (dm_giio a flag2 wp2) ((flag1 <= flag2) /\ hist_ord wp2 wp1) (fun _ -> True)
+let dm_giio_subcomp a flag1 flag2 wp1 wp2 f = 
+  admit ();
+  dm_iio_subcomp a wp1 wp2 f
+
+let dm_giio_if_then_else (a : Type u#a) (fl1 fl2:tflag)
+  (wp1 wp2: hist a) (f : dm_giio a fl1 wp1) (g : dm_giio a fl2 wp2) (b : bool) : Type =
+  dm_giio a (fl1 + fl2) (hist_if_then_else wp1 wp2 b)
+
 total
-reifiable
 reflectable
 effect {
-  IIOwp (a:Type) (wp : hist #event a) 
+  IIOwp (a:Type) (flag:erased tflag) (wp : hist #event a) 
   with {
-       repr       = dm_iio
-     ; return     = dm_iio_return
-     ; bind       = dm_iio_bind 
-     ; subcomp    = dm_iio_subcomp
-     ; if_then_else = dm_iio_if_then_else
+       repr       = dm_giio
+     ; return     = dm_giio_return
+     ; bind       = dm_giio_bind 
+     ; subcomp    = dm_giio_subcomp
+     ; if_then_else = dm_giio_if_then_else
      }
 }
 
-assume val __reify_IIOwp (#a:Type) (#wp:Hist.hist a) ($f:unit -> IIO.IIOwp a wp) : IIO.dm_iio a wp
+let dm_giio_partial_return 
+  (pre:pure_pre) : dm_giio (squash pre) NoActions (partial_call_wp pre) by (compute ()) =
+  dm_partial_return iio_cmds iio_sig event iio_wps pre
 
-sub_effect PURE ~> IIOwp = lift_pure_dm_iio
+val lift_pure_dm_giio :
+  a: Type ->
+  w: pure_wp a ->
+  f: (eqtype_as_type unit -> PURE a w) ->
+  Tot (dm_giio a NoActions (wp_lift_pure_hist w))
+let lift_pure_dm_giio a w f = 
+  lemma_wp_lift_pure_hist_implies_as_requires #a #event w;
+  FStar.Monotonic.Pure.elim_pure_wp_monotonicity_forall ();
+  let lhs : dm_giio _ NoActions _ = dm_giio_partial_return (as_requires w) in
+  let rhs = (fun (pre:(squash (as_requires w))) -> dm_giio_return a (f pre)) in
+  let m = dm_giio_bind _ _ NoActions NoActions _ _ lhs rhs in
+  dm_giio_subcomp a NoActions NoActions _ _ m
+  
+sub_effect PURE ~> IIOwp = lift_pure_dm_giio
 
 effect IIO
   (a:Type)
+  (fl:erased tflag)
   (pre : trace -> Type0)
   (post : trace -> a -> trace -> Type0) =
-  IIOwp a (to_hist pre post) 
-
+  IIOwp a fl (to_hist pre post) 
+  
 let static_cmd
   (cmd : io_cmds)
   (arg : io_sig.args cmd) :
-  IIO (io_resm cmd)
+  IIO (io_sig.res cmd arg) IOActions
     (requires (fun h -> io_pre cmd arg h))
     (ensures (fun h (r:io_sig.res cmd arg) lt ->
         lt == [convert_call_to_event cmd arg r])) =
   IIOwp?.reflect (iio_call cmd arg)
 
-let get_trace () : IIOwp trace (fun p h -> forall lt. lt == [] ==> p lt h) =
+let get_trace () : IIOwp trace GetTraceActions
+  (fun p h -> forall lt. lt == [] ==> p lt h) =
   IIOwp?.reflect (iio_call GetTrace ())
-*)
+
+private
+let performance_test (#fl:tflag) : IIOwp unit (fl+IOActions) (fun p h -> forall lt. (List.length lt == 6) \/ (List.length lt == 7) ==> p lt ()) =
+  let fd = static_cmd Openfile "../Makefile" in
+  let fd = static_cmd Openfile "../Makefile" in
+  let fd = static_cmd Openfile "../Makefile" in
+  let fd = static_cmd Openfile "../Makefile" in
+  let fd = static_cmd Openfile "../Makefile" in
+  let fd = static_cmd Openfile "../Makefile" in
+  if Inl? fd then let _ = static_cmd Close (Inl?.v fd) in () else 
+  ()
+
+(** ** Model compilation **)
+type rc_typ (t1:Type u#a) (t2:Type u#b) = t1 -> trace -> t2 -> trace -> bool
+
+type eff_rc_typ_cont (fl:erased tflag) (t1:Type u#a) (t2:Type u#b) (rc:rc_typ t1 t2) (x:t1) (initial_h:erased trace) =
+  y:t2 -> IIO ((erased trace) * bool) fl (fun h -> (initial_h `suffix_of` h)) (fun h (the_lt, b) lt -> apply_changes initial_h the_lt == h /\ lt == [] /\ (b <==> rc x initial_h y the_lt))
+  
+type eff_rc_typ (fl:erased tflag) (t1 t2:Type) (rc:rc_typ t1 t2) =
+  x:t1 -> IIO (initial_h:(erased trace) & eff_rc_typ_cont fl t1 t2 rc x initial_h) fl (fun _ -> True) (fun h (| initial_h, _ |) lt -> h == reveal initial_h /\ lt == [])
+
+let get_local_trace (h':trace) :
+  IIO trace GetTraceActions
+    (requires (fun h -> h' `suffix_of` h))
+    (ensures (fun h lt' lt ->
+      lt == [] /\
+      h == (apply_changes h' lt'))) =
+  let h = get_trace () in
+  suffix_of_length h' h;
+  let n : nat = (List.length h) - (List.length h') in
+  let (lt', ht) = List.Tot.Base.splitAt n h in
+  lemma_splitAt_equal n h;
+  lemma_splitAt_suffix h h';
+  List.Tot.Properties.rev_involutive lt';
+  assert (h == apply_changes h' (List.rev lt'));
+  List.rev lt'
+
+val enforce_rc : (#a:Type u#a) -> (#b:Type u#b) -> rc:rc_typ a b -> eff_rc_typ AllActions a b rc
+let enforce_rc #a #b rc x =
+  let initial_h = get_trace () in
+  let cont : eff_rc_typ_cont AllActions a b rc x (hide initial_h) = 
+    (fun y -> ( 
+      let lt = get_local_trace initial_h in 
+      (hide lt, rc x initial_h y lt))) in
+  (| hide initial_h, cont |)
+
+type pck_rc = (t1:Type u#a & t2:Type u#b & rc_typ t1 t2)
+type pck_eff_rc (fl:erased tflag) = pck:pck_rc & eff_rc_typ fl (Mkdtuple3?._1 pck) (Mkdtuple3?._2 pck) (Mkdtuple3?._3 pck)
+
+val make_rc_eff : pck_rc u#a u#b -> pck_eff_rc u#a u#b AllActions
+let make_rc_eff r = (| r, (enforce_rc (Mkdtuple3?._3 r)) |)
+
+type typ_posts (fl:erased tflag) (rcs:tree pck_rc) = 
+  posts:(tree (pck_eff_rc fl)){
+    equal_trees rcs (map_tree posts dfst)}
