io/old/Compiler.Languages.fst
@@ -1,0 +1,217 @@
+module Compiler.Languages
+
+open FStar.Tactics
+open FStar.Tactics.Typeclasses
+open FStar.Ghost
+
+open CommonUtils
+open TC.Monitorable.Hist
+
+(** ** IIO **)
+include IIO
+
+(** ** ILang **)
+(** ILang is a language that acts as an intermediate language between the rich IIO effect that has
+    rich types and pre- and post-conditions and an ML language as OCaml.
+
+    The task of compiling an IIO computation is big and it implies converting rich types and pre- and
+    post-conditions to runtime checks. Therefore, this intermediate language simplifies our work.
+    By compiling to this intermediate language, we convert all of this static requirments to dynamic checks
+    but we keep the post-conditions around enough to show that the computation preserves its trace
+    properties.
+
+    So, ILang is weakly typed and its computation can have only as post-condition that it respects a 
+    trace property. The pre-condition must be trivial.
+**)
+
+
+effect IIOpi (a:Type) (fl:FStar.Ghost.erased tflag) (pi : monitorable_prop) = 
+  IIOwp a fl (pi_as_hist #a pi)
+
+class ilang (t:Type u#a) (pi:monitorable_prop) = { [@@@no_method] mldummy : unit }
+
+instance ilang_unit (pi:monitorable_prop) : ilang unit pi = { mldummy = () }
+instance ilang_file_descr (pi:monitorable_prop) : ilang file_descr pi = { mldummy = () }
+
+instance ilang_bool (pi:monitorable_prop) : ilang bool pi = { mldummy = () }
+instance ilang_int (pi:monitorable_prop) : ilang int pi = { mldummy = () }
+instance ilang_option (pi:monitorable_prop) t1 {| d1:ilang t1 pi |} : ilang (option t1) pi =
+  { mldummy = () }
+instance ilang_pair (pi:monitorable_prop) t1 {| d1:ilang t1 pi |} t2 {| d2:ilang t2 pi |} : ilang (t1 * t2) pi = 
+  { mldummy = () }
+instance ilang_either (pi:monitorable_prop) t1 {| d1:ilang t1 pi |} t2 {| d2:ilang t2 pi |} : ilang (either t1 t2) pi =
+  { mldummy = () }
+instance ilang_resexn (pi:monitorable_prop) t1 {| d1:ilang t1 pi |} : ilang (resexn t1) pi =
+  { mldummy = () }
+
+type ilang_arrow_typ (fl:erased tflag) (t1 t2:Type) pi = t1 -> IIOpi t2 fl pi
+
+(** An ilang arrow is a statically verified arrow to respect pi.
+    It can expect an argument that respects a different pi1, or it
+    can return a function that respects pi2. 
+**)
+instance ilang_arrow (#fl:erased tflag) (#pi1 #pi2 pi:monitorable_prop) #t1 (d1:ilang t1 pi1) #t2 (d2:ilang t2 pi2) : ilang (ilang_arrow_typ fl t1 t2 pi) pi =
+  { mldummy = () }
+
+(**instance ilang_fo_uint8 : ilang_fo UInt8.t = { fo_pred = () }
+instance ilang_fo_string : ilang_fo string = { fo_pred = () }
+instance ilang_fo_bytes : ilang_fo Bytes.bytes = { fo_pred = () }
+instance ilang_fo_open_flag : ilang_fo open_flag = { fo_pred = () } 
+instance ilang_fo_socket_bool_option : ilang_fo socket_bool_option = { fo_pred = () }
+instance ilang_fo_file_descr : ilang_fo file_descr = { fo_pred = () }
+instance ilang_fo_zfile_perm : ilang_fo zfile_perm = { fo_pred = () }
+instance ilang_fo_pair_2 t1 t2 t3 {| ilang_fo t1 |} {| ilang_fo t2 |} {| ilang_fo t3 |} : ilang_fo (t1 * t2 * t3) = { fo_pred = () }
+instance ilang_fo_pair_3 t1 t2 t3 t4 {| ilang_fo t1 |} {| ilang_fo t2 |} {| ilang_fo t3 |} {| ilang_fo t4 |} : ilang_fo (t1 * t2 * t3 * t4) = { fo_pred = () }
+instance ilang_fo_option t1 {| ilang_fo t1 |} : ilang_fo (option t1) = { fo_pred = () }
+instance ilang_fo_list t1 {| ilang_fo t1 |} : ilang_fo (list t1) = { fo_pred = () } **)
+
+
+
+(** ** RILang **)
+
+class rilang (t:Type u#a) (pi:monitorable_prop) = { 
+  [@@@no_method]
+  mldummy : unit }
+
+instance rilang_unit (pi:monitorable_prop) : rilang unit pi = { mldummy = () }
+instance rilang_file_descr (pi:monitorable_prop) : rilang file_descr pi = { mldummy = () }
+
+instance rilang_bool (pi:monitorable_prop) : rilang bool pi = { mldummy = () }
+instance rilang_int (pi:monitorable_prop) : rilang int pi = { mldummy = () }
+instance rilang_option (pi:monitorable_prop) t1 {| d1:rilang t1 pi |} : rilang (option t1) pi =
+  { mldummy = () }
+instance rilang_pair (pi:monitorable_prop) t1 {| d1:rilang t1 pi |} t2 {| d2:rilang t2 pi |} : rilang (t1 * t2) pi = 
+  { mldummy = () }
+instance rilang_either (pi:monitorable_prop) t1 {| d1:rilang t1 pi |} t2 {| d2:rilang t2 pi |} : rilang (either t1 t2) pi =
+  { mldummy = () }
+instance rilang_resexn (pi:monitorable_prop) t1 {| d1:rilang t1 pi |} : rilang (resexn t1) pi =
+  { mldummy = () }
+
+type rilang_dm (pi:monitorable_prop) (a:Type) = c:(IO.Sig.iio a){pi_as_hist pi `Hist.hist_ord` IIO.dm_iio_theta c} 
+
+let as_rilang_dm (w:IIO.dm_iio 'a (pi_as_hist 'p)) : rilang_dm 'p 'a = w
+
+let as_iio_dm (w:rilang_dm 'p 'a) : IIO.dm_iio 'a (pi_as_hist 'p) = 
+  let tree : IO.Sig.iio 'a = w in
+  assert (pi_as_hist 'p `Hist.hist_ord` IIO.dm_iio_theta tree);
+  tree
+
+type rilang_arrow_typ (t1 t2:Type) pi = t1 -> rilang_dm pi t2
+
+instance rilang_arrow (#pi1 #pi2 pi:monitorable_prop) #t1 (d1:rilang t1 pi1) #t2 (d2:rilang t2 pi2) : rilang (rilang_arrow_typ t1 t2 pi) pi =
+  { mldummy = () }
+
+
+(** ** MLang **)
+noeq type monad = {
+  m    : Type u#a -> Type u#(max 1 a);
+  ret  : #a:Type -> a -> m a;
+  (* TODO: bind should be polymorphic in two universes *)
+  bind : #a:Type u#a -> #b:Type u#a -> m a -> (a -> m b) -> m b;
+  (* We don't want acts to be part of this monad because we want to provide different versions *)
+}
+
+val free : monad
+let free = { 
+  m = IO.Sig.iio; 
+  ret = IO.Sig.iio_return; 
+  bind = IO.Sig.iio_bind; 
+}
+
+type acts (mon:monad) = op:(Universe.raise_t IO.Sig.io_cmds) -> arg:IO.Sig.io_sig.args (Universe.downgrade_val op) -> mon.m (IO.Sig.io_sig.res (Universe.downgrade_val op) arg)
+
+(** **** Free Actions **)
+val free_acts : acts free
+let free_acts cmd arg = IO.Sig.Call.iio_call (Universe.downgrade_val cmd) arg
+
+let spec_free_acts (ca:acts free) =
+  (forall (cmd:IO.Sig.io_cmds) (arg:IO.Sig.io_sig.args cmd). IO.Sig.iio_wps cmd arg `Hist.hist_ord` IIO.dm_iio_theta (ca (Universe.raise_val cmd) arg))
+
+let lemma_free_acts () : Lemma (spec_free_acts free_acts) = 
+  assert (forall (cmd:IO.Sig.io_cmds) (arg:IO.Sig.io_sig.args cmd). IO.Sig.iio_wps cmd arg `Hist.hist_ord` IIO.dm_iio_theta (free_acts (Universe.raise_val cmd) arg));
+  assert (spec_free_acts free_acts) by (assumption ())
+
+(** ** MLang **)
+class mlang (t:Type u#a) = { [@@@no_method] mldummy : unit }
+
+(** *** FO instances **)
+instance mlang_unit : mlang unit = { mldummy = () }
+
+instance mlang_bool : mlang bool = { mldummy = () }
+instance mlang_int : mlang int = { mldummy = () }
+
+instance mlang_pair t1 t2 {| d1:mlang t1 |} {| d2:mlang t2 |} : mlang (t1 * t2) = 
+  { mldummy = () }
+instance mlang_either t1 t2 {| d1:mlang t1 |} {| d2:mlang t2 |} : mlang (either t1 t2) =
+  { mldummy = () }
+
+instance mlang_free_arrow #t1 #t2 (d1:mlang t1) (d2:mlang t2) : mlang (t1 -> free.m t2) =
+  { mldummy = () }
+
+instance mlang_effectpoly 
+  (#ct:(Type->Type)->Type)
+  (d1:mlang (ct free.m)) : 
+  mlang (mon:monad -> acts mon -> ct mon.m) =
+  { mldummy = () }
+
+let dm_mon (pi:monitorable_prop) : monad = {
+  m = rilang_dm pi;
+  ret = (fun (x:'a) -> IIO.dm_iio_return 'a x);
+  bind = (fun (m:rilang_dm pi 'a) (k:'a -> rilang_dm pi 'b) -> 
+    let wp : Hist.hist 'b = Hist.hist_bind (pi_as_hist #'a pi) (fun _ -> pi_as_hist pi) in 
+    let tr : IIO.dm_iio 'b wp = IIO.dm_iio_bind _ _ _ _ (as_iio_dm m) (fun x -> as_iio_dm (k x)) in
+    lemma_bind_pi_implies_pi #'a #'b pi;
+    let w = IIO.dm_iio_subcomp 'b wp (pi_as_hist pi) tr in
+    as_rilang_dm w)
+}
+
+assume val dm_acts (pi:monitorable_prop) : acts (dm_mon pi)
+
+
+(** *** Manual tests *)
+(** Manual tests of MLang. 
+    Types of programs that should be part of MLang:
+   - [v] int -> free.m int
+   - [ ] int -> free.m (int -> free.m int)
+   - [v] (int -> free.m int) -> free.m int (?)
+   - [v] mon:monad -> acts mon -> int -> mon.m int 
+   - [v] mon:monad -> acts mon -> (int -> mon.m int) -> mon.m int 
+   - [ ] mon:monad -> acts mon -> int -> mon.m (int -> mon.m int)
+   - [v] (mon:monad -> acts mon -> int -> mon.m int) -> free.m int
+   - [v] (mon:monad -> acts mon -> (int -> mon.m int) -> mon.m int) -> free.m int 
+
+   Types of programs that should not be part of MLang:
+   - [ ] how can I identify such cases?
+**)
+
+let test_mlang_free_arrow : mlang (int -> free.m int) =
+  mlang_free_arrow mlang_int mlang_int
+
+(** Cannot be typed because universe problems
+let test_mlang_free_arrow_rhs_ho : mlang (int (int -> free.m int) -> free.m int) =
+  mlang_free_arrow free.m mlang_int (mlang_free_arrow free.m mlang_int mlang_int)
+ **)
+
+let test_mlang_free_arrow_lhs_ho : mlang ((int -> free.m int) -> free.m int) =
+  mlang_free_arrow (mlang_free_arrow mlang_int mlang_int) mlang_int
+
+let test_mlang_fo_effectpoly : mlang (mon:monad -> acts mon -> int -> mon.m int) =
+  mlang_effectpoly #(fun m -> int -> m int) (mlang_free_arrow mlang_int mlang_int)
+
+let test_mlang_lhs_ho_effectpoly : mlang (mon:monad -> acts mon -> (int -> mon.m int) -> mon.m int) =
+  mlang_effectpoly #(fun m -> (int -> m int) -> m int) (mlang_free_arrow (mlang_free_arrow mlang_int mlang_int) mlang_int)
+
+(** This can not be typed because universe problems: 
+let test_mlang_rhs_ho_effectpoly : mlang (mon:monad -> acts mon -> int -> mon.m (int -> mon.m int)) = **)
+
+let test_mlang_prog1 : mlang ((mon:monad -> acts mon -> int -> mon.m int) -> free.m int) =
+  mlang_free_arrow
+    (mlang_effectpoly #(fun m -> int -> m int) (mlang_free_arrow mlang_int mlang_int))
+    mlang_int
+
+let test_mlang_prog2 : mlang ((mon:monad -> acts mon -> (int -> mon.m int) -> mon.m int) -> free.m int) =
+  mlang_free_arrow
+    (mlang_effectpoly 
+      #(fun m -> (int -> m int) -> m int)
+      (mlang_free_arrow (mlang_free_arrow mlang_int mlang_int) mlang_int))
+    mlang_int
