io/old/IIO.fst
@@ -1,0 +1,92 @@
+module IIO
+
+open FStar.Tactics
+open ExtraTactics
+open FStar.Calc
+
+open IO.Sig
+open IO.Sig.Call
+open DMFree
+
+(** The postcondition for an io computation is defined over the
+result (type: a) and local trace (type: trace).
+The local trace represents the events that happend during the
+computation. Local trace is in chronological order.
+
+We also have the history (type: trace) which represents the
+events that happend until the beggining of the io computation.
+The history is  in reverse chronology order.
+
+At the end of an io computation, the local trace is appended
+in reverse order to the history. **)
+let dm_iio_theta #a = theta #a #iio_cmds #iio_sig #event iio_wps
+  
+type dm_iio = dm iio_cmds iio_sig event iio_wps
+let dm_iio_return (a:Type) (x:a) : dm_iio a (hist_return x) =
+  dm_return iio_cmds iio_sig event iio_wps a x
+
+val dm_iio_bind  : 
+  a: Type ->
+  b: Type ->
+  wp_v: hist a ->
+  wp_f: (_: a -> hist b) ->
+  v: dm_iio a wp_v ->
+  f: (x: a -> dm_iio b (wp_f x)) ->
+  Tot (dm_iio b (hist_bind wp_v wp_f))
+let dm_iio_bind a b wp_v wp_f v f = dm_bind iio_cmds iio_sig event iio_wps a b wp_v wp_f v f
+
+val dm_iio_subcomp : 
+  a: Type ->
+  wp1: hist a ->
+  wp2: hist a ->
+  f: dm_iio a wp1 ->
+  Pure (dm_iio a wp2) (hist_ord wp2 wp1) (fun _ -> True)
+let dm_iio_subcomp a wp1 wp2 f = dm_subcomp iio_cmds iio_sig event iio_wps a wp1 wp2 f
+
+let dm_iio_if_then_else a wp1 wp2 f g b = dm_if_then_else iio_cmds iio_sig event iio_wps a wp1 wp2 f g b
+
+val lift_pure_dm_iio :
+  a: Type ->
+  w: pure_wp a ->
+  f: (eqtype_as_type unit -> PURE a w) ->
+  Tot (dm_iio a (wp_lift_pure_hist w))
+let lift_pure_dm_iio = lift_pure_dm iio_cmds iio_sig event iio_wps
+
+(*
+[@@allow_informative_binders]
+total
+reifiable
+reflectable
+effect {
+  IIOwp (a:Type) (wp : hist #event a) 
+  with {
+       repr       = dm_iio
+     ; return     = dm_iio_return
+     ; bind       = dm_iio_bind 
+     ; subcomp    = dm_iio_subcomp
+     ; if_then_else = dm_iio_if_then_else
+     }
+}
+
+assume val __reify_IIOwp (#a:Type) (#wp:Hist.hist a) ($f:unit -> IIO.IIOwp a wp) : IIO.dm_iio a wp
+
+sub_effect PURE ~> IIOwp = lift_pure_dm_iio
+
+effect IIO
+  (a:Type)
+  (pre : trace -> Type0)
+  (post : trace -> a -> trace -> Type0) =
+  IIOwp a (to_hist pre post) 
+
+let static_cmd
+  (cmd : io_cmds)
+  (arg : io_sig.args cmd) :
+  IIO (io_resm cmd)
+    (requires (fun h -> io_pre cmd arg h))
+    (ensures (fun h (r:io_sig.res cmd arg) lt ->
+        lt == [convert_call_to_event cmd arg r])) =
+  IIOwp?.reflect (iio_call cmd arg)
+
+let get_trace () : IIOwp trace (fun p h -> forall lt. lt == [] ==> p lt h) =
+  IIOwp?.reflect (iio_call GetTrace ())
+*)
